Iterator/Combinators/Drop.lean
@@ -16,25 +16,21 @@ structure Drop (α : Type u) where
   remaining : Nat
   inner : α
 
-instance [Monad m] [Iterator α m β] [SteppableIterator α m β] :
-    SimpleIterator (Drop α) m β where
+instance [Monad m] [Iterator α m β] : SimpleIterator (Drop α) m β where
+  αInternal := Drop (IterState α m)
+  βInternal := Iterator.βInternal α m
+  αEquiv := {
+      hom it := { inner := Iterator.αEquiv.hom it.inner, remaining := it.remaining }
+      inv it := { inner := Iterator.αEquiv.inv it.inner, remaining := it.remaining }
+      hom_inv := by simp [Equiv.hom_inv]
+      inv_hom := by simp [Equiv.inv_hom] }
+  βEquiv := Iterator.βEquiv
   step it := matchStep (m := m) it.inner
       (fun it' b => match it.remaining with
-        | 0 => pure <| .yield ⟨0, it'⟩ b ⟨⟩
+        | 0 => pure <| .yield ⟨0, it'⟩ (Iterator.βEquiv.hom b) ⟨⟩
         | remaining' + 1 => pure <| .skip ⟨remaining', it'⟩ ⟨⟩)
       (fun it' => pure <| .skip ⟨it.remaining, it'⟩ ⟨⟩)
       (pure <| .done ⟨⟩)
-
-instance [Monad m] [Iterator α m β] [SteppableIterator.{max u v x} α m β] [SteppableIterator.{max u v y} α m β] :
-    SimpleIterator.CompatibleUniverses.{x, y} (Drop α) m where
-  compatible it := by
-    simp [SimpleIterator.step]
-    simp only [matchStep, matchStepH, IterationT.bindH]
-    ext
-    rw [iff_iff_eq]
-    congr
-    ext
-    split <;> (try split) <;> rfl
 
 /--
 Given an iterator `it` and a natural number `n`, `it.drop n` is an iterator that forwards all of
@@ -62,13 +58,13 @@ _TODO_: prove `Productive`
 Currently, this combinator incurs an additional O(1) cost with each output of `it`, even when the iterator
 does not drop any elements anymore.
 -/
-def Iter.drop [Iterator α m β] [SteppableIterator α m β] [Monad m] (n : Nat) (it : Iter (α := α) m β) :=
-  toIter m <| Drop.mk n it.inner
+def Iter.drop [Iterator α m β] [Monad m] (n : Nat) (it : Iter (α := α) m β) :=
+  toIter (α := Drop α) m <| Drop.mk n it.inner
 
-def Drop.rel (m : Type w → Type w') [Iterator α m β] : Drop α → Drop α → Prop :=
+def Drop.rel (m : Type w → Type w') [Iterator α m β] : Drop (IterState α m) → Drop (IterState α m) → Prop :=
   InvImage FiniteIteratorWF.lt (finiteIteratorWF (m := m) ∘ Drop.inner)
 
-instance [Iterator α m β] [SteppableIterator α m β] [Monad m] [Finite α m] : SimpleIterator.Finite (Drop α) m where
+instance [Iterator α m β] [Monad m] [Finite α m] : SimpleIterator.Finite (Drop α) m where
   rel := Drop.rel m
   wf := by
     apply InvImage.wf
