Iterator/Combinators/Take.lean
@@ -21,11 +21,10 @@ instance [Monad m] [Iterator α m β] : SimpleIterator (Take α) m β where
   αInternal := Take (IterState α m)
   βInternal := Iterator.βInternal α m
   αEquiv := {
-    hom it := { inner := Iterator.αEquiv.hom it.inner, remaining := it.remaining }
-    inv it := { inner := Iterator.αEquiv.inv it.inner, remaining := it.remaining }
-    hom_inv := by simp [Equiv.hom_inv]
-    inv_hom := by simp [Equiv.inv_hom]
-  }
+      hom it := { inner := Iterator.αEquiv.hom it.inner, remaining := it.remaining }
+      inv it := { inner := Iterator.αEquiv.inv it.inner, remaining := it.remaining }
+      hom_inv := by simp [Equiv.hom_inv]
+      inv_hom := by simp [Equiv.inv_hom] }
   βEquiv := Iterator.βEquiv
   step it :=
     match it with
@@ -101,75 +100,3 @@ instance [Monad m] [Iterator α m β] [Productive α m] : SimpleIterator.Finite 
         apply Take.rel_of_inner
         exact hs
       · cases successor_done.mp h
-
-#exit
-
-variable {m} [Monad m] [Iterator α m β]
-
-instance [Iterator α m β] [Monad m] : Iterator (Take α) m β :=
-  Iteration.instIterator fun
-    | { remaining := 0, inner := _ } => pure <| .done ⟨⟩
-    | { remaining := remaining' + 1, inner := it } =>
-      matchStep it
-        (fun it' b => pure <| .yield ⟨remaining', it'⟩ b ⟨⟩)
-        (fun it' => pure <| .skip ⟨remaining' + 1, it'⟩ ⟨⟩)
-        (pure <| .done ⟨⟩)
-
-/--
-Given an iterator `it` and a natural number `n`, `it.take n` is an iterator that outputs
-up to the first `n` of `it`'s values in order and then terminates.
-
-**Marble diagram:**
-
-```text
-it          ---a----b---c--d-e--⊥
-it.take 3   ---a----b---c⊥
-
-it          ---a--⊥
-it.take 3   ---a--⊥
-```
-
-**Termination properties:**
-
-* `Finite` instance: always ✓
-* `Productive` instance: only if `it` is productive
-
-_TODO_: prove `Productive`
-
-**Performance:**
-
-This combinator incurs an additional O(1) cost with each output of `it`.
--/
-def Iter.take [Iterator α m β] [Monad m] (n : Nat) (it : Iter (α := α) m β) :=
-  toIter m <| Take.mk n it.inner
-
-def Take.rel (m : Type w → Type w') [Iterator α m β] : Take α → Take α → Prop :=
-  InvImage (Prod.Lex Nat.lt_wfRel.rel ProductiveIteratorWF.lt)
-    (fun it => (it.remaining, productiveIteratorWF (m := m) it.inner))
-
-theorem Take.rel_of_remaining [Iterator α m β] {it it' : Take α}
-    (h : it'.remaining < it.remaining) : Take.rel m it' it :=
-  Prod.Lex.left _ _ h
-
-theorem Take.rel_of_inner [Iterator α m β] {remaining : Nat} {it it' : α}
-    (h : (productiveIteratorWF (m := m) it').lt (productiveIteratorWF it)) :
-    Take.rel m ⟨remaining, it'⟩ ⟨remaining, it⟩ :=
-  Prod.Lex.right _ h
-
-instance [Iterator α m β] [Monad m] [Productive α m] : Finite (Take α) m := by
-  refine finite_instIterator _ (rel := Take.rel m) ?_ ?_
-  · apply InvImage.wf
-    refine ⟨fun (a, b) => Prod.lexAccessible (WellFounded.apply ?_ a) (WellFounded.apply ?_) b⟩
-    · exact WellFoundedRelation.wf
-    · exact Productive.wf
-  · intro it it' h
-    split at h
-    · cases up_successor_done.mp h
-    · obtain ⟨_, _, hy, h⟩ | ⟨_, hs, h⟩ | ⟨hd, h⟩ := prop_successor_matchStep h
-      · cases up_successor_yield.mp h
-        apply Take.rel_of_remaining
-        simp
-      · cases up_successor_skip.mp h
-        apply Take.rel_of_inner
-        exact hs
-      · cases up_successor_done.mp h
