Iterator/MWE.lean
@@ -18,18 +18,20 @@ where
 set_option pp.universes true in
 set_option pp.explicit true in
 set_option trace.compiler.ir.result true in
-set_option compiler.small 10 in
+set_option compiler.small 20 in
 def firstOfEach (l : List (List Nat)) :=
   let it := List.iter l Id |>.flatMap (List.iter · Id |>.take 1)
   go (it) 0
 where
   go it acc : Nat :=
     match it.step with
-    | .yield it' x _ => go it' (acc)
+    | .yield it' x _ => go it' (acc + x)
     | .skip it' _ => go it' acc
     | .done _ => acc
   termination_by it-- .terminationByFinite
   decreasing_by all_goals sorry
+
+#eval! firstOfEach [[1, 2], [3, 4]]
 
 set_option trace.compiler.ir.result true in
 set_option compiler.small 2 in
